src/program_proof/std_proof.v
@@ -2,9 +2,17 @@ From Perennial.Helpers Require Import List ModArith.
 
 From Goose.github_com.goose_lang Require Import std.
 
+From iris.algebra Require Import excl gset.
 From Perennial.program_proof Require Import proof_prelude.
 From Perennial.goose_lang.lib Require Import slice.typed_slice.
 
+Class multiparG Σ :=
+   { multiparG_auth :> inG Σ (gset_disjR nat);
+     multiparG_tok :> inG Σ (exclR unitO) }.
+Definition multiparΣ := #[GFunctor (gset_disjR nat); GFunctor (exclR unitO)].
+Global Instance subG_multiparΣ {Σ} :
+  subG multiparΣ Σ → multiparG Σ.
+Proof. solve_inG. Qed.
 
 Section goose_lang.
 Context `{hG: heapGS Σ, !ffi_semantics _ _, !ext_types _}.
@@ -145,6 +153,139 @@ Proof.
   rewrite bool_decide_eq_true.
   iIntros (<-%sum_nooverflow_l). wp_pures. iModIntro.
   iApply "HΦ". iPureIntro. done.
+Qed.
+
+Lemma wp_Multipar `{!multiparG Σ} (P Q : nat → iProp Σ) (num : u64) (op : val) :
+  □(∀ i : u64, ⌜int.Z i < int.Z num⌝ -∗ P (int.nat i) -∗ WP op #i {{ _, Q (int.nat i) }}) -∗
+  {{{ [∗ list] i ∈ seq 0 (int.nat num), P i }}}
+    Multipar #num op
+  {{{ RET #(); [∗ list] i ∈ seq 0 (int.nat num), Q i }}}.
+Proof.
+  iIntros "#Hop !> %Φ HPs HΦ". wp_lam.
+  wp_apply wp_ref_to. { val_ty. }
+  iIntros (nleft_l) "Hnleft". wp_pures.
+  iMod (own_alloc (GSet (set_seq 0 (int.nat num)))) as (γpending) "Hpending".
+  { done. }
+  iMod (own_alloc (Excl ())) as (γtok) "Htok".
+  { done. }
+  set lock_inv := ( (∃ nleft : u64, nleft_l ↦[uint64T] #nleft ∗ own γtok (Excl ())) ∨
+    ∃ (nleft : u64) (pending : gset nat),
+      "%Hsz" ∷ ⌜size pending = int.nat nleft⌝ ∗
+      "Hnleft" ∷ nleft_l ↦[uint64T] #nleft ∗
+      "HPQ" ∷ ([∗ list] i ∈ seq 0 (int.nat num), ⌜i ∈ pending⌝ ∨ own γpending (GSet {[i]}) ∗ Q i)
+      )%I.
+  wp_apply (newlock_spec nroot _ lock_inv with "[Hnleft]").
+  { iModIntro. rewrite /lock_inv. iRight.
+    iExists num, (set_seq 0 (int.nat num)). iFrame. iSplit.
+    - iPureIntro. rewrite -list_to_set_seq size_list_to_set ?seq_length //.
+      apply NoDup_seq.
+    - iApply big_sepL_intro. iIntros "!> %k %i %Hlk". iLeft. iPureIntro.
+      apply elem_of_set_seq. apply lookup_seq in Hlk. lia. }
+  iIntros (lk) "#Hlk". wp_pures.
+  wp_apply (wp_newCond with "Hlk").
+  iIntros (cond) "#Hcond". wp_pures.
+  (* Loop starts *)
+  wp_apply wp_ref_to. { val_ty. }
+  iIntros (i_l) "Hi".
+  set loop_inv := (λ cur : u64,
+    [∗ list] i ∈ seq (int.nat cur) (int.nat num - int.nat cur)%nat, own γpending (GSet {[i]}) ∗ P i)%I.
+  wp_apply (wp_forUpto loop_inv _ _ 0 with "[] [HPs Hpending Hi]").
+  { word. }
+  { clear Φ.
+    iIntros "%cur !> %Φ (Hloop & Hcur & %Hcur) HΦ". wp_pures.
+    wp_load.
+    iAssert (loop_inv (word.add cur 1) ∗ own γpending (GSet {[int.nat cur]}) ∗ P (int.nat cur))%I with "[Hloop]"
+      as "(Hloop & Hpending & HP)".
+    { rewrite /loop_inv.
+      replace (int.nat num - int.nat cur)%nat with (1 + (int.nat num - int.nat (word.add cur 1)))%nat by word.
+      rewrite seq_app. simpl.
+      iDestruct "Hloop" as "(($ & $) & Hloop)".
+      replace (int.nat cur + 1)%nat with (int.nat (word.add cur 1)) by word.
+      done. }
+    wp_apply (wp_fork with "[HP Hpending]").
+    { iModIntro. wp_bind (op _). iApply (wp_wand with "[HP]").
+      { iApply "Hop"; done. }
+      iIntros (_v) "HQ". wp_pures. clear _v.
+      wp_apply (acquire_spec with "Hlk").
+      iIntros "(Hlocked & [Hinv|Hinv])".
+      { (* supposedly the main thread already removed all the resources...
+           this cannot really happen, but we just go along with it. *)
+        iDestruct "Hinv" as (nleft) "(Hnleft & Htok)".
+        wp_load. wp_store.
+        wp_apply (wp_condSignal with "Hcond").
+        wp_apply (release_spec with "[$Hlocked $Hlk Hnleft Htok]"); last done.
+        iLeft. eauto with iFrame. }
+      iNamed "Hinv".
+      wp_load. wp_store.
+      wp_apply (wp_condSignal with "Hcond").
+      wp_apply (release_spec with "[-]"); last done. iFrame "Hlocked Hlk".
+      iRight. iExists _, (pending ∖ {[int.nat cur]}). iFrame "Hnleft".
+      iDestruct (big_sepL_lookup_acc_impl (int.nat cur) (int.nat cur) with "HPQ") as "[Hcur Hclose]".
+      { rewrite lookup_seq. word. }
+      iFreeze "Hclose".
+      iDestruct "Hcur" as "[%Hpending|[Hpending2 _]]"; last first.
+      { (* This index is supposedly already done -- contradiction. *)
+        iDestruct (own_valid_2 with "Hpending Hpending2") as %Hval%gset_disj_valid_op.
+        exfalso. set_solver. }
+      iModIntro. iSplit.
+      { iPureIntro. trans (size (pending) - size (C:=gset nat) ({[int.nat cur]}))%nat.
+        - (* TODO use size_difference once upstream std++ MR 324 lands *)
+          rewrite {2}(union_difference {[int.nat cur]} pending); last set_solver.
+          rewrite size_union; last by set_solver+. lia.
+        - rewrite Hsz size_singleton.
+          assert (int.nat nleft ≠ 0%nat). 2:word.
+          rewrite -Hsz. intros Hemp%size_empty_inv.
+          rewrite ->Hemp in Hpending. set_solver. }
+      iThaw "Hclose". iApply "Hclose"; last by eauto with iFrame.
+      iIntros "!> %i' %i %Hi %Hnotcur [%Hpend|Hdone]".
+      - iLeft. iPureIntro. apply lookup_seq in Hi as [-> ?]. set_solver.
+      - iRight. eauto. }
+    wp_pures. iApply "HΦ". eauto with iFrame. }
+  { (* loop invariant holds initially *)
+    iFrame "Hi". rewrite /loop_inv.
+    replace (int.nat num - int.nat 0%Z)%nat with (int.nat num) by word.
+    iClear "#". clear loop_inv lock_inv.
+    change (int.nat 0) with 0%nat.
+    remember 0%nat as start eqn:Hstart. clear Hstart.
+    iInduction (int.nat num) as [|n] "IH" forall (start); clear num; simpl.
+    { done. }
+    iDestruct "HPs" as "[$ HPs]".
+    rewrite -gset_disj_union; last first.
+    { apply disjoint_singleton_l.
+      rewrite elem_of_set_seq. lia. }
+    iDestruct "Hpending" as "[$ Hpending]".
+    iApply ("IH" with "HPs Hpending"). }
+  (* continuation after loop *)
+  iIntros "_".
+  wp_apply (acquire_spec with "Hlk").
+  iIntros "[Hlocked Hinv]". wp_pures.
+  wp_apply (wp_forBreak_cond' with "[-]"); first iNamedAccu.
+  iIntros "!> Hloop". iNamed "Hloop".
+  iDestruct "Hinv" as "[Hinv|Hinv]".
+  { (* Supposedly we already took out everything, but now we have the token twice -- contradiction. *)
+    iDestruct "Hinv" as (?) "[_ Htok2]".
+    iDestruct (own_valid_2 with "Htok Htok2") as %[]. }
+  iNamed "Hinv".
+  wp_load. wp_pures.
+  case_bool_decide as Hleft; wp_pures.
+  { (* Not yet done, once more around the loop. *)
+    wp_apply (wp_condWait with "[$Hcond $Hlk $Hlocked Hnleft HPQ]").
+    { rewrite /lock_inv. eauto 10 with iFrame. }
+    iIntros "[Hlocked Hinv]". wp_pures.
+    eauto 10 with iFrame. }
+  iModIntro. iRight. iSplit; first done.
+  wp_apply (release_spec with "[$Hlk $Hlocked Hnleft Htok]").
+  { rewrite /lock_inv. iLeft. eauto 10 with iFrame. }
+  iApply "HΦ".
+  iApply (big_sepL_impl with "HPQ").
+  iIntros "!> %i' %i %Hlk [%Hpending|[_ $]]".
+  exfalso.
+  apply Znot_lt_ge in Hleft.
+  change (int.Z 0) with 0 in Hleft.
+  assert (int.nat nleft = 0%nat) as Hnotleft by word.
+  rewrite Hnotleft in Hsz.
+  apply size_empty_inv in Hsz.
+  set_solver.
 Qed.
 
 End goose_lang.
